reorganize chacha20 example

examples/riscv/chacha20/chacha20_specScript.sml
@@ -33,436 +33,63 @@ open program_logicSimps;
 open bir_env_oldTheory;
 open bir_program_varsTheory;
 
-val _ = new_theory "chacha_spec";
+open chachaTheory;
 
-(* ------------- *)
-(* ChaCha theory *)
-(* ------------- *)
+val _ = new_theory "chacha20_spec";
 
-(*
-op line (a:idx) (b:idx) (d:idx) (s:int) (m:state) : state =
-  let m = m.[a <- (m.[a] + m.[b])] in
-  let m = m.[d <- W32.rol (m.[d] +^ m.[a]) s] in m.
-*)
+(* ChaCha spec *)
 
-Definition chacha_line:
- chacha_line (a:word32) (b:word32) (d:word32) (s:word32)
-  (m:word32 -> word32) =
-  let m = (a =+ (m a) + (m b)) m in
-  let m = (d =+ ((m d) ?? (m a)) #<<~ s) m in
-  m
-End
-
-Definition chacha_line_alt:
- chacha_line_alt (a:word32) (b:word32) (d:word32) (s:word32)
-  (m:word32 -> word32) =
- let m = (a =+ (m a) + (m b)) m in
- let m = (d =+ (((m d) ?? (m a)) <<~ s) || (((m d) ?? (m a)) >>>~ (32w - s))) m in
- m
-End
-
-Theorem word32_le_31_eq:
- !(w:word32). w <=+ 31w ==> 31w && w = w
-Proof
- blastLib.BBLAST_TAC
-QED
-
-Theorem replace_word_rol_bv_or_shifts:
- !x s : word32. s <=+ 31w ==>
-  x #<<~ s = (x <<~ s) || (x >>>~ (32w - s))
-Proof
- rw [] >>
- `dimindex (:32) = 2 ** 5` by rw [] >>
- MP_TAC (Q.SPECL [`5`, `x`, `s`] (INST_TYPE [Type.alpha |-> ``:32``] word_rol_OR_SHIFT)) >>
- rw [word32_le_31_eq]
-QED
-
-Theorem chacha_line_expand:
- !a b d s m. s <=+ 31w ==>
-  chacha_line a b d s m = 
-   (let m = (a =+ (m a) + (m b)) m in
-    let m = (d =+ (((m d) ?? (m a)) <<~ s) || (((m d) ?? (m a)) >>>~ (32w - s))) m
-    in m)  
-Proof
- rw [chacha_line,replace_word_rol_bv_or_shifts]
-QED
-
-Theorem chacha_line_alt_eq:
- !a b d s m. s <=+ 31w ==>
-  chacha_line a b d s m = chacha_line_alt a b d s m
-Proof
- rw [chacha_line_expand,chacha_line_alt]
-QED
-
-(*
-op quarter_round a b c d : shuffle =
-  line a b d 16 \oo
-  line c d b 12 \oo
-  line a b d 8  \oo
-  line c d b 7.
-*)
-
-Definition chacha_quarter_round:
- chacha_quarter_round (a:word32) (b:word32) (c:word32) (d:word32) =
-  chacha_line c d b 7w o
-  chacha_line a b d 8w o 
-  chacha_line c d b 12w o 
-  chacha_line a b d 16w
-End
-
-Definition chacha_quarter_round_alt:
- chacha_quarter_round_alt (a:word32) (b:word32) (c:word32) (d:word32) =
-  chacha_line_alt c d b 7w o
-  chacha_line_alt a b d 8w o 
-  chacha_line_alt c d b 12w o 
-  chacha_line_alt a b d 16w
-End
-
-Theorem chacha_quarter_round_alt_eq:
- !a b c d m.
- chacha_quarter_round a b c d m = 
- chacha_quarter_round_alt a b c d m
-Proof
- rw [chacha_quarter_round,chacha_quarter_round_alt] >>
- `(7w:word32) <=+ 31w` by rw [] >>
- `(8w:word32) <=+ 31w` by rw [] >>
- `(12w:word32) <=+ 31w` by rw [] >>
- `(16w:word32) <=+ 31w` by rw [] >>
- rw [chacha_line_alt_eq]
-QED
-
-(*
-op column_round : shuffle =
-  quarter_round 0 4 8  12 \oo
-  quarter_round 1 5 9  13 \oo
-  quarter_round 2 6 10 14 \oo
-  quarter_round 3 7 11 15.
-*)
-        
-Definition chacha_column_round:
- chacha_column_round =
-  chacha_quarter_round 3w 7w 11w 15w o
-  chacha_quarter_round 2w 6w 10w 14w o
-  chacha_quarter_round 1w 5w 9w 13w o
-  chacha_quarter_round 0w 4w 8w 12w
-End
-
-Definition chacha_column_round_alt:
- chacha_column_round_alt =
-  chacha_quarter_round_alt 3w 7w 11w 15w o
-  chacha_quarter_round_alt 2w 6w 10w 14w o
-  chacha_quarter_round_alt 1w 5w 9w 13w o
-  chacha_quarter_round_alt 0w 4w 8w 12w
-End
-
-Theorem chacha_column_round_alt_eq:
- !m. chacha_column_round m = chacha_column_round_alt m
-Proof
- rw [chacha_column_round,chacha_column_round_alt] >>
- rw [chacha_quarter_round_alt_eq]
-QED
-
-(*
-op diagonal_round : shuffle =
-  quarter_round 0 5 10 15 \oo
-  quarter_round 1 6 11 12 \oo
-  quarter_round 2 7 8  13 \oo
-  quarter_round 3 4 9  14.
-*)
-
-Definition chacha_diagonal_round:
- chacha_diagonal_round =
-  chacha_quarter_round 3w 4w 9w 14w o
-  chacha_quarter_round 2w 7w 8w 13w o
-  chacha_quarter_round 1w 6w 11w 12w o
-  chacha_quarter_round 0w 5w 10w 15w
-End
-
-Definition chacha_diagonal_round_alt:
- chacha_diagonal_round_alt =
-  chacha_quarter_round_alt 3w 4w 9w 14w o
-  chacha_quarter_round_alt 2w 7w 8w 13w o
-  chacha_quarter_round_alt 1w 6w 11w 12w o
-  chacha_quarter_round_alt 0w 5w 10w 15w
-End
-
-Theorem chacha_diagonal_round_alt_eq:
- !m. chacha_diagonal_round m = chacha_diagonal_round_alt m
-Proof
- rw [chacha_diagonal_round,chacha_diagonal_round_alt] >>
- rw [chacha_quarter_round_alt_eq]
-QED
-
-(*
-op double_round: shuffle =
-  column_round \oo diagonal_round.
-*)
-
-Definition chacha_double_round:
- chacha_double_round =
-  chacha_diagonal_round o chacha_column_round
-End
-
-Definition chacha_double_round_alt:
- chacha_double_round_alt =
-  chacha_diagonal_round_alt o chacha_column_round_alt
-End
-
-Theorem chacha_double_round_alt_eq:
- !m. chacha_double_round m = chacha_double_round_alt m
-Proof
- rw [chacha_double_round,chacha_double_round_alt] >>
- rw [chacha_diagonal_round_alt_eq,chacha_column_round_alt_eq]
-QED
-
-Definition chacha_rounds:
- chacha_rounds =
-  chacha_double_round o
-  chacha_double_round o
-  chacha_double_round o
-  chacha_double_round o
-  chacha_double_round o
-  chacha_double_round o
-  chacha_double_round o
-  chacha_double_round o
-  chacha_double_round o
-  chacha_double_round
-End
-
-Definition chacha_rounds_alt:
- chacha_rounds_alt =
-  chacha_double_round_alt o
-  chacha_double_round_alt o
-  chacha_double_round_alt o
-  chacha_double_round_alt o
-  chacha_double_round_alt o
-  chacha_double_round_alt o
-  chacha_double_round_alt o
-  chacha_double_round_alt o
-  chacha_double_round_alt o
-  chacha_double_round_alt
-End
-
-Theorem chacha_rounds_alt_eq:
- !m. chacha_rounds m = chacha_rounds_alt m
-Proof
- rw [chacha_rounds,chacha_rounds_alt] >>
- rw [chacha_double_round_alt_eq]
-QED
-
-Definition chacha_add_16:
- chacha_add_16 (s: word32 -> word32)
-  (s' : word32 -> word32) : word32 -> word32 =
-  let m = s in
-  let m = (0w =+ (s 0w) + (s' 0w)) m in
-  let m = (1w =+ (s 1w) + (s' 1w)) m in
-  let m = (2w =+ (s 2w) + (s' 2w)) m in
-  let m = (3w =+ (s 3w) + (s' 3w)) m in
-  let m = (4w =+ (s 4w) + (s' 4w)) m in
-  let m = (5w =+ (s 5w) + (s' 5w)) m in
-  let m = (6w =+ (s 6w) + (s' 6w)) m in
-  let m = (7w =+ (s 7w) + (s' 7w)) m in
-  let m = (8w =+ (s 8w) + (s' 8w)) m in
-  let m = (9w =+ (s 9w) + (s' 9w)) m in
-  let m = (10w =+ (s 10w) + (s' 10w)) m in
-  let m = (11w =+ (s 11w) + (s' 11w)) m in
-  let m = (12w =+ (s 12w) + (s' 12w)) m in
-  let m = (13w =+ (s 13w) + (s' 13w)) m in
-  let m = (14w =+ (s 14w) + (s' 14w)) m in
-  let m = (15w =+ (s 15w) + (s' 15w)) m in
-  m
-End
-
-Definition chacha_core:
- chacha_core (s:word32 -> word32) : word32 -> word32 =
-  let s' = chacha_rounds s in
-  chacha_add_16 s' s
-End
-
-Definition chacha_core_alt:
- chacha_core_alt (s:word32 -> word32) : word32 -> word32 =
-  let s' = chacha_rounds_alt s in
-  chacha_add_16 s' s
-End
-
-Theorem chacha_core_alt_eq:
- !s. chacha_core s = chacha_core_alt s
-Proof
- rw [chacha_core,chacha_core_alt] >>
- rw [chacha_rounds_alt_eq]
-QED
-
-Definition chacha_setup:
- chacha_setup (m : word32 -> word32) 
-  (k : word32 -> word32) (n : word32 -> word32) (c : word32) 
-   : word32 -> word32 =
-  let m = (0w =+ 0x61707865w) m in
-  let m = (1w =+ 0x3320646ew) m in
-  let m = (2w =+ 0x79622d32w) m in
-  let m = (3w =+ 0x6b206574w) m in
-  let m = (4w =+ (k 0w)) m in
-  let m = (5w =+ (k 1w)) m in
-  let m = (6w =+ (k 2w)) m in
-  let m = (7w =+ (k 3w)) m in
-  let m = (8w =+ (k 4w)) m in
-  let m = (9w =+ (k 5w)) m in
-  let m = (10w =+ (k 6w)) m in
-  let m = (11w =+ (k 7w)) m in
-  let m = (12w =+ c) m in
-  let m = (13w =+ (n 0w)) m in
-  let m = (14w =+ (n 1w)) m in
-  let m = (15w =+ (n 2w)) m in
-  m
-End
-
-(* Examples and validation *)
-
-Definition chacha_example_state_row:
- chacha_example_state_row : word32 -> word32 =
-  let m = ARB in
-  let m = (0w =+ 0x11111111w) m in
-  let m = (1w =+ 0x01020304w) m in
-  let m = (2w =+ 0x9b8d6f43w) m in
-  let m = (3w =+ 0x01234567w) m in
-  m
-End
-
-Definition chacha_example_state_full:
- chacha_example_state_full : word32 -> word32 =
-  let m = ARB in
-  let m = (0w =+ 0x879531e0w) m in
-  let m = (1w =+ 0xc5ecf37dw) m in
-  let m = (2w =+ 0x516461b1w) m in
-  let m = (3w =+ 0xc9a62f8aw) m in
-  let m = (4w =+ 0x44c20ef3w) m in
-  let m = (5w =+ 0x3390af7fw) m in
-  let m = (6w =+ 0xd9fc690bw) m in
-  let m = (7w =+ 0x2a5f714cw) m in
-  let m = (8w =+ 0x53372767w) m in
-  let m = (9w =+ 0xb00a5631w) m in
-  let m = (10w =+ 0x974c541aw) m in
-  let m = (11w =+ 0x359e9963w) m in
-  let m = (12w =+ 0x5c971061w) m in
-  let m = (13w =+ 0x3d631689w) m in
-  let m = (14w =+ 0x2098d9d6w) m in
-  let m = (15w =+ 0x91dbd320w) m in
-  m
-End
-
-(* RFC7539 2.1.1 example *)
-Theorem chacha_example_quarter_round_row[local]:
- chacha_quarter_round 0w 1w 2w 3w chacha_example_state_row 0w = 0xea2a92f4w
- /\
- chacha_quarter_round 0w 1w 2w 3w chacha_example_state_row 1w = 0xcb1cf8cew
- /\
- chacha_quarter_round 0w 1w 2w 3w chacha_example_state_row 2w = 0x4581472ew
- /\
- chacha_quarter_round 0w 1w 2w 3w chacha_example_state_row 3w = 0x5881c4bbw
-Proof
- EVAL_TAC
-QED
-
-(* RFC7539 2.2.1 example *)
-Theorem chacha_example_quarter_round_full[local]:
- chacha_quarter_round 2w 7w 8w 13w chacha_example_state_full 2w = 0xbdb886dcw
- /\
- chacha_quarter_round 2w 7w 8w 13w chacha_example_state_full 7w = 0xcfacafd2w
- /\
- chacha_quarter_round 2w 7w 8w 13w chacha_example_state_full 8w = 0xe46bea80w
- /\
- chacha_quarter_round 2w 7w 8w 13w chacha_example_state_full 13w = 0xccc07c79w
-Proof
- EVAL_TAC
-QED
-
-Definition chacha_example_state_key_setup:
- chacha_example_state_key_setup : word32 -> word32 =
-  let m = ARB in
-  let m = (0w =+ 0x61707865w) m in
-  let m = (1w =+ 0x3320646ew) m in
-  let m = (2w =+ 0x79622d32w) m in
-  let m = (3w =+ 0x6b206574w) m in
-  let m = (4w =+ 0x03020100w) m in
-  let m = (5w =+ 0x07060504w) m in
-  let m = (6w =+ 0x0b0a0908w) m in
-  let m = (7w =+ 0x0f0e0d0cw) m in
-  let m = (8w =+ 0x13121110w) m in
-  let m = (9w =+ 0x17161514w) m in
-  let m = (10w =+ 0x1b1a1918w) m in
-  let m = (11w =+ 0x1f1e1d1cw) m in
-  let m = (12w =+ 0x00000001w) m in
-  let m = (13w =+ 0x09000000w) m in
-  let m = (14w =+ 0x4a000000w) m in
-  let m = (15w =+ 0x00000000w) m in
-  m
-End
-
-(* RFC7539 2.3.2 example *)
-Theorem chacha_example_state_key_setup[local]:
- chacha_rounds chacha_example_state_key_setup 0w = 0x837778abw
- /\
- chacha_rounds chacha_example_state_key_setup 1w = 0xe238d763w
- /\
- chacha_rounds chacha_example_state_key_setup 2w = 0xa67ae21ew
- /\
- chacha_rounds chacha_example_state_key_setup 3w = 0x5950bb2fw
-Proof
- EVAL_TAC
-QED
-
-(* RISC-V spec *)
-
-Definition riscv_chacha_line_exp_fst_def:
- riscv_chacha_line_exp_fst (pre_a:word32) (pre_b:word32) : word32 =
+Definition chacha_line_exp_fst_def:
+ chacha_line_exp_fst (pre_a:word32) (pre_b:word32) : word32 =
   pre_a + pre_b
 End
 
-Definition riscv_chacha_line_exp_snd_spec_def:
- riscv_chacha_line_exp_snd_spec pre_a pre_d (s:word32) : word32 =
+Definition chacha_line_exp_snd_orig_def:
+ chacha_line_exp_snd_orig pre_a pre_d (s:word32) : word32 =
   (pre_a ?? pre_d) #<<~ s
 End
 
-Definition riscv_chacha_line_exp_snd_def:
- riscv_chacha_line_exp_snd pre_a pre_d (s:word32) : word32 =
+Definition chacha_line_exp_snd_def:
+ chacha_line_exp_snd pre_a pre_d (s:word32) : word32 =
   ((pre_a ?? pre_d) <<~ s) || ((pre_a ?? pre_d) >>>~ (32w - s))
 End
 
-Theorem riscv_chacha_line_exp_snd_spec_eq:
-!(a:word32) (d:word32) (s:word32). s <=+ 31w ==>
- riscv_chacha_line_exp_snd_spec a d s = riscv_chacha_line_exp_snd a d s
+Theorem chacha_line_exp_snd_orig_eq:
+ !(a:word32) (d:word32) (s:word32). s <=+ 31w ==>
+  chacha_line_exp_snd_orig a d s = chacha_line_exp_snd a d s
 Proof
  rw [
-  riscv_chacha_line_exp_snd_spec_def,
-  riscv_chacha_line_exp_snd_def,
+  chacha_line_exp_snd_orig_def,
+  chacha_line_exp_snd_def,
   replace_word_rol_bv_or_shifts  
  ]
 QED
 
-Definition riscv_chacha_quarter_round_exprs_def:
- riscv_chacha_quarter_round_exprs pre_a pre_b pre_c pre_d
+Definition chacha_quarter_round_exprs_def:
+ chacha_quarter_round_exprs pre_a pre_b pre_c pre_d
   : word32 # word32 # word32 # word32 =
   let a = pre_a in
   let b = pre_b in
   let c = pre_c in
   let d = pre_d in
 
-  let a = riscv_chacha_line_exp_fst a b in
-  let d = riscv_chacha_line_exp_snd a d 16w in
+  let a = chacha_line_exp_fst a b in
+  let d = chacha_line_exp_snd a d 16w in
 
-  let c = riscv_chacha_line_exp_fst c d in
-  let b = riscv_chacha_line_exp_snd c b 12w in
+  let c = chacha_line_exp_fst c d in
+  let b = chacha_line_exp_snd c b 12w in
 
-  let a = riscv_chacha_line_exp_fst a b in
-  let d = riscv_chacha_line_exp_snd a d 8w in
+  let a = chacha_line_exp_fst a b in
+  let d = chacha_line_exp_snd a d 8w in
 
-  let c = riscv_chacha_line_exp_fst c d in
-  let b = riscv_chacha_line_exp_snd c b 7w in
+  let c = chacha_line_exp_fst c d in
+  let b = chacha_line_exp_snd c b 7w in
 
   (a,b,c,d)
 End
 
-Definition riscv_chacha_column_round_exprs_def:
- riscv_chacha_column_round_exprs 
+Definition chacha_column_round_exprs_def:
+ chacha_column_round_exprs 
   pre_arr_0 pre_arr_1 pre_arr_2 pre_arr_3
   pre_arr_4 pre_arr_5 pre_arr_6 pre_arr_7
   pre_arr_8 pre_arr_9 pre_arr_10 pre_arr_11
@@ -473,23 +100,23 @@ Definition riscv_chacha_column_round_exprs_def:
    word32 # word32 # word32 # word32
   =
  let (arr_0,arr_4,arr_8,arr_12) =
-   riscv_chacha_quarter_round_exprs pre_arr_0 pre_arr_4 pre_arr_8 pre_arr_12
+   chacha_quarter_round_exprs pre_arr_0 pre_arr_4 pre_arr_8 pre_arr_12
  in
  let (arr_1,arr_5,arr_9,arr_13) =
-   riscv_chacha_quarter_round_exprs pre_arr_1 pre_arr_5 pre_arr_9 pre_arr_13
+   chacha_quarter_round_exprs pre_arr_1 pre_arr_5 pre_arr_9 pre_arr_13
  in
  let (arr_2,arr_6,arr_10,arr_14) =
-   riscv_chacha_quarter_round_exprs pre_arr_2 pre_arr_6 pre_arr_10 pre_arr_14
+   chacha_quarter_round_exprs pre_arr_2 pre_arr_6 pre_arr_10 pre_arr_14
  in
  let (arr_3,arr_7,arr_11,arr_15) =
-   riscv_chacha_quarter_round_exprs pre_arr_3 pre_arr_7 pre_arr_11 pre_arr_15
+   chacha_quarter_round_exprs pre_arr_3 pre_arr_7 pre_arr_11 pre_arr_15
  in
  (arr_0,arr_1,arr_2,arr_3,arr_4,arr_5,arr_6,arr_7,
   arr_8,arr_9,arr_10,arr_11,arr_12,arr_13,arr_14,arr_15)
 End
 
-Definition riscv_chacha_diagonal_round_exprs_def:
- riscv_chacha_diagonal_round_exprs 
+Definition chacha_diagonal_round_exprs_def:
+ chacha_diagonal_round_exprs 
   pre_arr_0 pre_arr_1 pre_arr_2 pre_arr_3
   pre_arr_4 pre_arr_5 pre_arr_6 pre_arr_7
   pre_arr_8 pre_arr_9 pre_arr_10 pre_arr_11
@@ -500,16 +127,16 @@ Definition riscv_chacha_diagonal_round_exprs_def:
    word32 # word32 # word32 # word32
   =
  let (arr_0,arr_5,arr_10,arr_15) =
-   riscv_chacha_quarter_round_exprs pre_arr_0 pre_arr_5 pre_arr_10 pre_arr_15
+   chacha_quarter_round_exprs pre_arr_0 pre_arr_5 pre_arr_10 pre_arr_15
  in
  let (arr_1,arr_6,arr_11,arr_12) =
-   riscv_chacha_quarter_round_exprs pre_arr_1 pre_arr_6 pre_arr_11 pre_arr_12
+   chacha_quarter_round_exprs pre_arr_1 pre_arr_6 pre_arr_11 pre_arr_12
  in
  let (arr_2,arr_7,arr_8,arr_13) =
-   riscv_chacha_quarter_round_exprs pre_arr_2 pre_arr_7 pre_arr_8 pre_arr_13
+   chacha_quarter_round_exprs pre_arr_2 pre_arr_7 pre_arr_8 pre_arr_13
  in
  let (arr_3,arr_4,arr_9,arr_14) =
-   riscv_chacha_quarter_round_exprs pre_arr_3 pre_arr_4 pre_arr_9 pre_arr_14
+   chacha_quarter_round_exprs pre_arr_3 pre_arr_4 pre_arr_9 pre_arr_14
  in
  (arr_0,arr_1,arr_2,arr_3,arr_4,arr_5,arr_6,arr_7,
   arr_8,arr_9,arr_10,arr_11,arr_12,arr_13,arr_14,arr_15)
@@ -517,26 +144,25 @@ End
 
 (* RISC-V single line contract *)
 
-Definition riscv_chacha_line_pre_def:
- riscv_chacha_line_pre (pre_a:word32) (pre_b:word32) (pre_d:word32)
+Definition riscv_chacha20_line_pre_def:
+ riscv_chacha20_line_pre (pre_a:word32) (pre_b:word32) (pre_d:word32)
   (m:riscv_state) : bool =
  (n2w (w2n (m.c_gpr m.procID 10w)) = pre_a /\
   n2w (w2n (m.c_gpr m.procID 22w)) = pre_b /\
   n2w (w2n (m.c_gpr m.procID 26w)) = pre_d)
 End
 
-Definition riscv_chacha_line_post_def:
- riscv_chacha_line_post (pre_a:word32) (pre_b:word32) (pre_d:word32)
+Definition riscv_chacha20_line_post_def:
+ riscv_chacha20_line_post (pre_a:word32) (pre_b:word32) (pre_d:word32)
   (m:riscv_state) : bool =
- (n2w (w2n (m.c_gpr m.procID 20w)) = riscv_chacha_line_exp_fst pre_a pre_b /\
-  n2w (w2n (m.c_gpr m.procID 10w)) =
-   riscv_chacha_line_exp_snd (riscv_chacha_line_exp_fst pre_a pre_b) pre_d 16w)
+ (n2w (w2n (m.c_gpr m.procID 20w)) = chacha_line_exp_fst pre_a pre_b /\
+  n2w (w2n (m.c_gpr m.procID 10w)) = chacha_line_exp_snd (chacha_line_exp_fst pre_a pre_b) pre_d 16w)
 End
 
 (* RISC-V single quarter round contract *)
 
-Definition riscv_chacha_quarter_round_pre_def:
- riscv_chacha_quarter_round_pre (pre_a:word32) (pre_b:word32) (pre_c:word32) (pre_d:word32)
+Definition riscv_chacha20_quarter_round_pre_def:
+ riscv_chacha20_quarter_round_pre (pre_a:word32) (pre_b:word32) (pre_c:word32) (pre_d:word32)
   (m:riscv_state) : bool =
   (n2w (w2n (m.c_gpr m.procID 10w)) = pre_a /\
    n2w (w2n (m.c_gpr m.procID 22w)) = pre_b /\
@@ -544,10 +170,10 @@ Definition riscv_chacha_quarter_round_pre_def:
    n2w (w2n (m.c_gpr m.procID 26w)) = pre_d)
 End
 
-Definition riscv_chacha_quarter_round_post_def:
- riscv_chacha_quarter_round_post (pre_a:word32) (pre_b:word32) (pre_c:word32) (pre_d:word32)
+Definition riscv_chacha20_quarter_round_post_def:
+ riscv_chacha20_quarter_round_post (pre_a:word32) (pre_b:word32) (pre_c:word32) (pre_d:word32)
   (m:riscv_state) : bool =
-  (let (a,b,c,d) = riscv_chacha_quarter_round_exprs pre_a pre_b pre_c pre_d in
+  (let (a,b,c,d) = chacha_quarter_round_exprs pre_a pre_b pre_c pre_d in
    n2w (w2n (m.c_gpr m.procID 20w)) = a /\
    n2w (w2n (m.c_gpr m.procID 21w)) = b /\
    n2w (w2n (m.c_gpr m.procID 8w)) = c /\
@@ -556,8 +182,8 @@ End
 
 (* RISC-V column round contract *)
 
-Definition riscv_chacha_column_round_pre_def:
- riscv_chacha_column_round_pre 
+Definition riscv_chacha20_column_round_pre_def:
+ riscv_chacha20_column_round_pre 
   (pre_arr_0:word32) (pre_arr_1:word32) (pre_arr_2:word32) (pre_arr_3:word32)
   (pre_arr_4:word32) (pre_arr_5:word32) (pre_arr_6:word32) (pre_arr_7:word32) 
   (pre_arr_8:word32) (pre_arr_9:word32) (pre_arr_10:word32) (pre_arr_11:word32) 
@@ -566,7 +192,7 @@ Definition riscv_chacha_column_round_pre_def:
  (n2w (w2n (m.c_gpr m.procID 10w)) = pre_arr_0 /\
   n2w (w2n (m.c_gpr m.procID 16w)) = pre_arr_1 /\
   n2w (w2n (m.c_gpr m.procID 17w)) = pre_arr_2 /\
-  n2w (w2n (m.c_gpr m.procID 6w)) = pre_arr_3 /\
+  n2w (w2n (m.c_gpr m.procID 6w))  = pre_arr_3 /\
   n2w (w2n (m.c_gpr m.procID 22w)) = pre_arr_4 /\
   n2w (w2n (m.c_gpr m.procID 11w)) = pre_arr_5 /\
   n2w (w2n (m.c_gpr m.procID 13w)) = pre_arr_6 /\
@@ -581,8 +207,8 @@ Definition riscv_chacha_column_round_pre_def:
   n2w (w2n (m.c_gpr m.procID 23w)) = pre_arr_15)
 End
 
-Definition riscv_chacha_column_round_post_def:
- riscv_chacha_column_round_post
+Definition riscv_chacha20_column_round_post_def:
+ riscv_chacha20_column_round_post
   (pre_arr_0:word32) (pre_arr_1:word32) (pre_arr_2:word32) (pre_arr_3:word32)
   (pre_arr_4:word32) (pre_arr_5:word32) (pre_arr_6:word32) (pre_arr_7:word32) 
   (pre_arr_8:word32) (pre_arr_9:word32) (pre_arr_10:word32) (pre_arr_11:word32) 
@@ -590,7 +216,7 @@ Definition riscv_chacha_column_round_post_def:
  (m:riscv_state) : bool =
  (let (arr_0,arr_1,arr_2,arr_3,arr_4,arr_5,arr_6,arr_7,arr_8,
        arr_9,arr_10,arr_11,arr_12,arr_13,arr_14,arr_15) =
-   riscv_chacha_column_round_exprs
+   chacha_column_round_exprs
      pre_arr_0 pre_arr_1 pre_arr_2 pre_arr_3 pre_arr_4 pre_arr_5 pre_arr_6 pre_arr_7
      pre_arr_8 pre_arr_9 pre_arr_10 pre_arr_11 pre_arr_12 pre_arr_13 pre_arr_14 pre_arr_15
   in
@@ -614,8 +240,8 @@ End
 
 (* RISC-V diagonal round contract *)
 
-Definition riscv_chacha_diagonal_round_pre_def:
- riscv_chacha_diagonal_round_pre 
+Definition riscv_chacha20_diagonal_round_pre_def:
+ riscv_chacha20_diagonal_round_pre 
   (pre_arr_0:word32) (pre_arr_1:word32) (pre_arr_2:word32) (pre_arr_3:word32)
   (pre_arr_4:word32) (pre_arr_5:word32) (pre_arr_6:word32) (pre_arr_7:word32) 
   (pre_arr_8:word32) (pre_arr_9:word32) (pre_arr_10:word32) (pre_arr_11:word32) 
@@ -639,8 +265,8 @@ Definition riscv_chacha_diagonal_round_pre_def:
   n2w (w2n (m.c_gpr m.procID 16w)) = pre_arr_15)
 End
 
-Definition riscv_chacha_diagonal_round_post_def:
- riscv_chacha_diagonal_round_post
+Definition riscv_chacha20_diagonal_round_post_def:
+ riscv_chacha20_diagonal_round_post
   (pre_arr_0:word32) (pre_arr_1:word32) (pre_arr_2:word32) (pre_arr_3:word32)
   (pre_arr_4:word32) (pre_arr_5:word32) (pre_arr_6:word32) (pre_arr_7:word32) 
   (pre_arr_8:word32) (pre_arr_9:word32) (pre_arr_10:word32) (pre_arr_11:word32) 
@@ -648,7 +274,7 @@ Definition riscv_chacha_diagonal_round_post_def:
  (m:riscv_state) : bool =
  (let (arr_0,arr_1,arr_2,arr_3,arr_4,arr_5,arr_6,arr_7,arr_8,
        arr_9,arr_10,arr_11,arr_12,arr_13,arr_14,arr_15) =
-   riscv_chacha_diagonal_round_exprs
+   chacha_diagonal_round_exprs
      pre_arr_0 pre_arr_1 pre_arr_2 pre_arr_3 pre_arr_4 pre_arr_5 pre_arr_6 pre_arr_7
      pre_arr_8 pre_arr_9 pre_arr_10 pre_arr_11 pre_arr_12 pre_arr_13 pre_arr_14 pre_arr_15
   in
@@ -672,8 +298,8 @@ End
 
 (* BIR spec *)
 
-Definition bspec_var_equal_32_lowcast_64_def:
- bspec_var_equal_32_lowcast_64 var exp =
+Definition bir_var_equal_32_lowcast_64_def:
+ bir_var_equal_32_lowcast_64 var exp =
   BExp_BinPred
    BIExp_Equal
    (BExp_Cast BIExp_LowCast (BExp_Den (BVar var (BType_Imm Bit64))) Bit32)
@@ -681,14 +307,14 @@ Definition bspec_var_equal_32_lowcast_64_def:
 End
 
 (* a =+ (m a) + (m b) *)
-Definition bspec_chacha_line_bir_exp_fst_def:
- bspec_chacha_line_bir_exp_fst pre_a_exp pre_b_exp : bir_exp_t =
+Definition chacha_line_bir_exp_fst_def:
+ chacha_line_bir_exp_fst pre_a_exp pre_b_exp : bir_exp_t =
   BExp_BinExp BIExp_Plus pre_a_exp pre_b_exp
 End
 
 (* d =+ (((m d) ?? (m a)) <<~ s) || (((m d) ?? (m a)) >>>~ (32w - s)) *)
-Definition bspec_chacha_line_bir_exp_snd_def:
- bspec_chacha_line_bir_exp_snd pre_a_exp pre_d_exp (s:word32) : bir_exp_t =
+Definition chacha_line_bir_exp_snd_def:
+ chacha_line_bir_exp_snd pre_a_exp pre_d_exp (s:word32) : bir_exp_t =
    BExp_BinExp BIExp_Or
      (BExp_BinExp BIExp_LeftShift 
       (BExp_BinExp BIExp_Xor pre_a_exp pre_d_exp)
@@ -698,31 +324,31 @@ Definition bspec_chacha_line_bir_exp_snd_def:
       (BExp_Const (Imm32 (32w-s))))
 End
 
-Definition bspec_chacha_quarter_round_bir_exprs_def:
- bspec_chacha_quarter_round_bir_exprs pre_a_exp pre_b_exp pre_c_exp pre_d_exp
+Definition chacha_quarter_round_bir_exprs_def:
+ chacha_quarter_round_bir_exprs pre_a_exp pre_b_exp pre_c_exp pre_d_exp
   : bir_exp_t # bir_exp_t # bir_exp_t # bir_exp_t =
   let a = pre_a_exp in
   let b = pre_b_exp in
   let c = pre_c_exp in
   let d = pre_d_exp in
 
-  let a = bspec_chacha_line_bir_exp_fst a b in
-  let d = bspec_chacha_line_bir_exp_snd a d 16w in
+  let a = chacha_line_bir_exp_fst a b in
+  let d = chacha_line_bir_exp_snd a d 16w in
 
-  let c = bspec_chacha_line_bir_exp_fst c d in
-  let b = bspec_chacha_line_bir_exp_snd c b 12w in
+  let c = chacha_line_bir_exp_fst c d in
+  let b = chacha_line_bir_exp_snd c b 12w in
     
-  let a = bspec_chacha_line_bir_exp_fst a b in
-  let d = bspec_chacha_line_bir_exp_snd a d 8w in
+  let a = chacha_line_bir_exp_fst a b in
+  let d = chacha_line_bir_exp_snd a d 8w in
 
-  let c = bspec_chacha_line_bir_exp_fst c d in
-  let b = bspec_chacha_line_bir_exp_snd c b 7w in
+  let c = chacha_line_bir_exp_fst c d in
+  let b = chacha_line_bir_exp_snd c b 7w in
 
   (a,b,c,d)
 End
 
-Definition bspec_chacha_column_round_bir_exprs_def:
- bspec_chacha_column_round_bir_exprs 
+Definition chacha_column_round_bir_exprs_def:
+ chacha_column_round_bir_exprs 
   pre_arr_0 pre_arr_1 pre_arr_2 pre_arr_3
   pre_arr_4 pre_arr_5 pre_arr_6 pre_arr_7
   pre_arr_8 pre_arr_9 pre_arr_10 pre_arr_11
@@ -733,23 +359,23 @@ Definition bspec_chacha_column_round_bir_exprs_def:
    bir_exp_t # bir_exp_t # bir_exp_t # bir_exp_t
   =
  let (arr_0,arr_4,arr_8,arr_12) =
-   bspec_chacha_quarter_round_bir_exprs pre_arr_0 pre_arr_4 pre_arr_8 pre_arr_12
+   chacha_quarter_round_bir_exprs pre_arr_0 pre_arr_4 pre_arr_8 pre_arr_12
  in
  let (arr_1,arr_5,arr_9,arr_13) =
-   bspec_chacha_quarter_round_bir_exprs pre_arr_1 pre_arr_5 pre_arr_9 pre_arr_13
+   chacha_quarter_round_bir_exprs pre_arr_1 pre_arr_5 pre_arr_9 pre_arr_13
  in
  let (arr_2,arr_6,arr_10,arr_14) =
-   bspec_chacha_quarter_round_bir_exprs pre_arr_2 pre_arr_6 pre_arr_10 pre_arr_14
+   chacha_quarter_round_bir_exprs pre_arr_2 pre_arr_6 pre_arr_10 pre_arr_14
  in
  let (arr_3,arr_7,arr_11,arr_15) =
-   bspec_chacha_quarter_round_bir_exprs pre_arr_3 pre_arr_7 pre_arr_11 pre_arr_15
+   chacha_quarter_round_bir_exprs pre_arr_3 pre_arr_7 pre_arr_11 pre_arr_15
  in
  (arr_0,arr_1,arr_2,arr_3,arr_4,arr_5,arr_6,arr_7,
   arr_8,arr_9,arr_10,arr_11,arr_12,arr_13,arr_14,arr_15)
 End
 
-Definition bspec_chacha_diagonal_round_bir_exprs_def:
- bspec_chacha_diagonal_round_bir_exprs 
+Definition chacha_diagonal_round_bir_exprs_def:
+ chacha_diagonal_round_bir_exprs 
   pre_arr_0 pre_arr_1 pre_arr_2 pre_arr_3
   pre_arr_4 pre_arr_5 pre_arr_6 pre_arr_7
   pre_arr_8 pre_arr_9 pre_arr_10 pre_arr_11
@@ -760,23 +386,23 @@ Definition bspec_chacha_diagonal_round_bir_exprs_def:
    bir_exp_t # bir_exp_t # bir_exp_t # bir_exp_t
   =
  let (arr_0,arr_5,arr_10,arr_15) =
-   bspec_chacha_quarter_round_bir_exprs pre_arr_0 pre_arr_5 pre_arr_10 pre_arr_15
+   chacha_quarter_round_bir_exprs pre_arr_0 pre_arr_5 pre_arr_10 pre_arr_15
  in
  let (arr_1,arr_6,arr_11,arr_12) =
-   bspec_chacha_quarter_round_bir_exprs pre_arr_1 pre_arr_6 pre_arr_11 pre_arr_12
+   chacha_quarter_round_bir_exprs pre_arr_1 pre_arr_6 pre_arr_11 pre_arr_12
  in
  let (arr_2,arr_7,arr_8,arr_13) =
-   bspec_chacha_quarter_round_bir_exprs pre_arr_2 pre_arr_7 pre_arr_8 pre_arr_13
+   chacha_quarter_round_bir_exprs pre_arr_2 pre_arr_7 pre_arr_8 pre_arr_13
  in
  let (arr_3,arr_4,arr_9,arr_14) =
-   bspec_chacha_quarter_round_bir_exprs pre_arr_3 pre_arr_4 pre_arr_9 pre_arr_14
+   chacha_quarter_round_bir_exprs pre_arr_3 pre_arr_4 pre_arr_9 pre_arr_14
  in
  (arr_0,arr_1,arr_2,arr_3,arr_4,arr_5,arr_6,arr_7,
   arr_8,arr_9,arr_10,arr_11,arr_12,arr_13,arr_14,arr_15)
 End
 
-Definition bspec_chacha_round_bir_exprs_def:
- bspec_chacha_round_bir_exprs 
+Definition chacha_double_round_bir_exprs_def:
+ chacha_double_round_bir_exprs 
   pre_arr_0 pre_arr_1 pre_arr_2 pre_arr_3
   pre_arr_4 pre_arr_5 pre_arr_6 pre_arr_7
   pre_arr_8 pre_arr_9 pre_arr_10 pre_arr_11
@@ -788,7 +414,7 @@ Definition bspec_chacha_round_bir_exprs_def:
   =
   let (arr_0,arr_1,arr_2,arr_3,arr_4,arr_5,arr_6,arr_7,
        arr_8,arr_9,arr_10,arr_11,arr_12,arr_13,arr_14,arr_15) =
-   bspec_chacha_column_round_bir_exprs
+   chacha_column_round_bir_exprs
     pre_arr_0 pre_arr_1 pre_arr_2 pre_arr_3
     pre_arr_4 pre_arr_5 pre_arr_6 pre_arr_7
     pre_arr_8 pre_arr_9 pre_arr_10 pre_arr_11
@@ -797,7 +423,7 @@ Definition bspec_chacha_round_bir_exprs_def:
 
   let (arr_0,arr_1,arr_2,arr_3,arr_4,arr_5,arr_6,arr_7,
        arr_8,arr_9,arr_10,arr_11, arr_12,arr_13,arr_14,arr_15) =
-   bspec_chacha_diagonal_round_bir_exprs
+   chacha_diagonal_round_bir_exprs
     arr_0 arr_1 arr_2 arr_3 arr_4 arr_5 arr_6 arr_7
     arr_8 arr_9 arr_10 arr_11 arr_12 arr_13 arr_14 arr_15
   in
@@ -812,96 +438,96 @@ End
 
 (* keysetup *)
 
-Definition chacha_keysetup_init_addr_def:
- chacha_keysetup_init_addr : word64 = 0x10488w
+Definition chacha20_keysetup_init_addr_def:
+ chacha20_keysetup_init_addr : word64 = 0x10488w
 End
 
-Definition chacha_keysetup_end_addr_def:
- chacha_keysetup_end_addr : word64 = (*0x106a8w*) 0x1053cw
+Definition chacha20_keysetup_end_addr_def:
+ chacha20_keysetup_end_addr : word64 = (*0x106a8w*) 0x1053cw
 End
 
 (* ivsetup *)
 
-Definition chacha_ivsetup_init_addr_def:
- chacha_ivsetup_init_addr : word64 = 0x106bcw
+Definition chacha20_ivsetup_init_addr_def:
+ chacha20_ivsetup_init_addr : word64 = 0x106bcw
 End
 
-Definition chacha_ivsetup_end_addr_def:
- chacha_ivsetup_end_addr : word64 = 0x10778w
+Definition chacha20_ivsetup_end_addr_def:
+ chacha20_ivsetup_end_addr : word64 = 0x10778w
 End
 
 (* first line *)
 
-Definition chacha_line_init_addr_def:
-  chacha_line_init_addr : word64 = 0x108a0w
+Definition chacha20_line_init_addr_def:
+  chacha20_line_init_addr : word64 = 0x108a0w
 End
 
-Definition chacha_line_end_addr_def:
- chacha_line_end_addr : word64 = 0x108b4w
+Definition chacha20_line_end_addr_def:
+ chacha20_line_end_addr : word64 = 0x108b4w
 End
 
 (* second line *)
 
-Definition chacha_other_line_init_addr_def:
-  chacha_other_line_init_addr : word64 = 0x108b4w
+Definition chacha20_other_line_init_addr_def:
+  chacha20_other_line_init_addr : word64 = 0x108b4w
 End
 
-Definition chacha_other_line_end_addr_def:
- chacha_other_line_end_addr : word64 = 0x108c8w
+Definition chacha20_other_line_end_addr_def:
+ chacha20_other_line_end_addr : word64 = 0x108c8w
 End
 
 (* first quarter round *)
 
-Definition chacha_quarter_round_init_addr_def:
-  chacha_quarter_round_init_addr : word64 = 0x108a0w
+Definition chacha20_quarter_round_init_addr_def:
+  chacha20_quarter_round_init_addr : word64 = 0x108a0w
 End
 
-Definition chacha_quarter_round_end_addr_def:
-  chacha_quarter_round_end_addr : word64 = 0x108f0w
+Definition chacha20_quarter_round_end_addr_def:
+  chacha20_quarter_round_end_addr : word64 = 0x108f0w
 End
 
 (* column round *)
 
-Definition chacha_column_round_init_addr_def:
-  chacha_column_round_init_addr : word64 = 0x108a0w
+Definition chacha20_column_round_init_addr_def:
+  chacha20_column_round_init_addr : word64 = 0x108a0w
 End
 
-Definition chacha_column_round_end_addr_def:
-  chacha_column_round_end_addr : word64 = 0x109e0w
+Definition chacha20_column_round_end_addr_def:
+  chacha20_column_round_end_addr : word64 = 0x109e0w
 End
 
 (* diagonal round *)
 
-Definition chacha_diagonal_round_init_addr_def:
-  chacha_diagonal_round_init_addr : word64 = 0x109e0w
+Definition chacha20_diagonal_round_init_addr_def:
+  chacha20_diagonal_round_init_addr : word64 = 0x109e0w
 End
 
-Definition chacha_diagonal_round_end_addr_def:
-  chacha_diagonal_round_end_addr : word64 = 0x10b64w
+Definition chacha20_diagonal_round_end_addr_def:
+  chacha20_diagonal_round_end_addr : word64 = 0x10b64w
 End
 
 (* double round loop body *)
 
-Definition chacha_double_round_init_addr_def:
-  chacha_double_round_init_addr : word64 = 0x108a0w
+Definition chacha20_double_round_init_addr_def:
+  chacha20_double_round_init_addr : word64 = 0x108a0w
 End
 
-Definition chacha_double_round_end_addr_def:
-  chacha_double_round_end_addr : word64 = 0x10b64w
+Definition chacha20_double_round_end_addr_def:
+  chacha20_double_round_end_addr : word64 = 0x10b64w
 End
 
 (* double round loop branch *)
 
-Definition chacha_double_round_branch_init_addr_def:
-  chacha_double_round_branch_init_addr : word64 = 0x10b64w
+Definition chacha20_double_round_branch_init_addr_def:
+  chacha20_double_round_branch_init_addr : word64 = 0x10b64w
 End
 
-Definition chacha_double_round_branch_end_addr_loop_def:
-  chacha_double_round_branch_end_addr_loop : word64 = 0x108a0w
+Definition chacha20_double_round_branch_end_addr_loop_def:
+  chacha20_double_round_branch_end_addr_loop : word64 = 0x108a0w
 End
 
-Definition chacha_double_round_branch_end_addr_continue_def:
-  chacha_double_round_branch_end_addr_continue : word64 = 0x10b68w
+Definition chacha20_double_round_branch_end_addr_continue_def:
+  chacha20_double_round_branch_end_addr_continue : word64 = 0x10b68w
 End
 
 (* --------------- *)
@@ -910,31 +536,31 @@ End
 
 (* keysetup *)
 
-val bspec_chacha_keysetup_pre_tm = bslSyntax.bandl [
+val bspec_chacha20_keysetup_pre_tm = bslSyntax.bandl [
   mem_addrs_aligned_prog_disj_bir_tm mem_params_standard "x10",
   mem_addrs_aligned_prog_disj_bir_tm mem_params_standard "x11"
 ];
 
-Definition bspec_chacha_keysetup_pre_def:
- bspec_chacha_keysetup_pre : bir_exp_t =
-  ^bspec_chacha_keysetup_pre_tm
+Definition bspec_chacha20_keysetup_pre_def:
+ bspec_chacha20_keysetup_pre : bir_exp_t =
+  ^bspec_chacha20_keysetup_pre_tm
 End
 
 (* ivsetup *)
 
-val bspec_chacha_ivsetup_pre_tm = bslSyntax.bandl [
+val bspec_chacha20_ivsetup_pre_tm = bslSyntax.bandl [
   mem_addrs_aligned_prog_disj_bir_tm mem_params_standard "x10",
   mem_addrs_aligned_prog_disj_bir_tm mem_params_standard "x11"
 ];
 
-Definition bspec_chacha_ivsetup_pre_def:
- bspec_chacha_ivsetup_pre : bir_exp_t =
-  ^bspec_chacha_ivsetup_pre_tm
+Definition bspec_chacha20_ivsetup_pre_def:
+ bspec_chacha20_ivsetup_pre : bir_exp_t =
+  ^bspec_chacha20_ivsetup_pre_tm
 End
 
 (* first line *)
 
-val bspec_chacha_line_pre_tm = bslSyntax.bandl [
+val bspec_chacha20_line_pre_tm = bslSyntax.bandl [
   ``BExp_BinPred
     BIExp_Equal
     (BExp_Cast BIExp_LowCast (BExp_Den (BVar "x10" (BType_Imm Bit64))) Bit32)
@@ -949,31 +575,31 @@ val bspec_chacha_line_pre_tm = bslSyntax.bandl [
     (BExp_Const (Imm32 pre_d))``  
 ];
 
-Definition bspec_chacha_line_pre_def:
- bspec_chacha_line_pre (pre_a:word32) (pre_b:word32) (pre_d:word32) : bir_exp_t =
-  ^bspec_chacha_line_pre_tm
+Definition bspec_chacha20_line_pre_def:
+ bspec_chacha20_line_pre (pre_a:word32) (pre_b:word32) (pre_d:word32) : bir_exp_t =
+  ^bspec_chacha20_line_pre_tm
 End
 
-val bspec_chacha_line_post_tm = bslSyntax.bandl [
+val bspec_chacha20_line_post_tm = bslSyntax.bandl [
   (snd o dest_eq o concl)
-   (EVAL ``bspec_var_equal_32_lowcast_64 "x20"
-    (bspec_chacha_line_bir_exp_fst
+   (EVAL ``bir_var_equal_32_lowcast_64 "x20"
+    (chacha_line_bir_exp_fst
      (BExp_Const (Imm32 pre_a)) (BExp_Const (Imm32 pre_b)))``),
   (snd o dest_eq o concl)
-   (EVAL ``bspec_var_equal_32_lowcast_64 "x10"
-    (bspec_chacha_line_bir_exp_snd
-     (bspec_chacha_line_bir_exp_fst (BExp_Const (Imm32 pre_a)) (BExp_Const (Imm32 pre_b)))
+   (EVAL ``bir_var_equal_32_lowcast_64 "x10"
+    (chacha_line_bir_exp_snd
+     (chacha_line_bir_exp_fst (BExp_Const (Imm32 pre_a)) (BExp_Const (Imm32 pre_b)))
      (BExp_Const (Imm32 pre_d)) 16w)``)
 ];
 
-Definition bspec_chacha_line_post_def:
- bspec_chacha_line_post (pre_a:word32) (pre_b:word32) (pre_d:word32) : bir_exp_t =
-  ^bspec_chacha_line_post_tm
+Definition bspec_chacha20_line_post_def:
+ bspec_chacha20_line_post (pre_a:word32) (pre_b:word32) (pre_d:word32) : bir_exp_t =
+  ^bspec_chacha20_line_post_tm
 End
 
 (* second line *)
 
-val bspec_chacha_line_pre_other_tm = bslSyntax.bandl [
+val bspec_chacha20_line_pre_other_tm = bslSyntax.bandl [
   ``BExp_BinPred
     BIExp_Equal
     (BExp_Cast BIExp_LowCast (BExp_Den (BVar "x10" (BType_Imm Bit64))) Bit32)
@@ -988,31 +614,31 @@ val bspec_chacha_line_pre_other_tm = bslSyntax.bandl [
     (BExp_Const (Imm32 pre_a))``  
 ];
 
-Definition bspec_chacha_line_pre_other_def:
- bspec_chacha_line_pre_other (pre_a:word32) (pre_b:word32) (pre_d:word32) : bir_exp_t =
-  ^bspec_chacha_line_pre_other_tm
+Definition bspec_chacha20_line_pre_other_def:
+ bspec_chacha20_line_pre_other (pre_a:word32) (pre_b:word32) (pre_d:word32) : bir_exp_t =
+  ^bspec_chacha20_line_pre_other_tm
 End
 
-val bspec_chacha_line_post_other_tm = bslSyntax.bandl [
+val bspec_chacha20_line_post_other_tm = bslSyntax.bandl [
   (snd o dest_eq o concl)
-   (EVAL ``bspec_var_equal_32_lowcast_64 "x8"
-    (bspec_chacha_line_bir_exp_fst
+   (EVAL ``bir_var_equal_32_lowcast_64 "x8"
+    (chacha_line_bir_exp_fst
      (BExp_Const (Imm32 pre_a)) (BExp_Const (Imm32 pre_b)))``),
   (snd o dest_eq o concl)
-   (EVAL ``bspec_var_equal_32_lowcast_64 "x15"
-    (bspec_chacha_line_bir_exp_snd
-     (bspec_chacha_line_bir_exp_fst (BExp_Const (Imm32 pre_a)) (BExp_Const (Imm32 pre_b)))
+   (EVAL ``bir_var_equal_32_lowcast_64 "x15"
+    (chacha_line_bir_exp_snd
+     (chacha_line_bir_exp_fst (BExp_Const (Imm32 pre_a)) (BExp_Const (Imm32 pre_b)))
      (BExp_Const (Imm32 pre_d)) 12w)``)
 ];
 
-Definition bspec_chacha_line_post_other_def:
- bspec_chacha_line_post_other (pre_a:word32) (pre_b:word32) (pre_d:word32) : bir_exp_t =
-  ^bspec_chacha_line_post_other_tm
+Definition bspec_chacha20_line_post_other_def:
+ bspec_chacha20_line_post_other (pre_a:word32) (pre_b:word32) (pre_d:word32) : bir_exp_t =
+  ^bspec_chacha20_line_post_other_tm
 End
 
 (* first quarter round *)
 
-val bspec_chacha_quarter_round_pre_tm = bslSyntax.bandl [
+val bspec_chacha20_quarter_round_pre_tm = bslSyntax.bandl [
   ``BExp_BinPred
     BIExp_Equal
     (BExp_Cast BIExp_LowCast (BExp_Den (BVar "x10" (BType_Imm Bit64))) Bit32)
@@ -1031,16 +657,16 @@ val bspec_chacha_quarter_round_pre_tm = bslSyntax.bandl [
     (BExp_Const (Imm32 pre_d))``  
 ];
 
-Definition bspec_chacha_quarter_round_pre_def:
- bspec_chacha_quarter_round_pre (pre_a:word32) (pre_b:word32)
+Definition bspec_chacha20_quarter_round_pre_def:
+ bspec_chacha20_quarter_round_pre (pre_a:word32) (pre_b:word32)
  (pre_c:word32) (pre_d:word32) : bir_exp_t =
-  ^bspec_chacha_quarter_round_pre_tm
+  ^bspec_chacha20_quarter_round_pre_tm
 End
 
-val bspec_chacha_quarter_round_post_tm =
+val bspec_chacha20_quarter_round_post_tm =
  let
    val bir_exprs = (snd o dest_eq o concl)
-    (EVAL ``bspec_chacha_quarter_round_bir_exprs 
+    (EVAL ``chacha_quarter_round_bir_exprs 
      (BExp_Const (Imm32 pre_a)) (BExp_Const (Imm32 pre_b))
      (BExp_Const (Imm32 pre_c)) (BExp_Const (Imm32 pre_d))``);
    val (a_exp, bir_exprs) = dest_pair bir_exprs;
@@ -1049,25 +675,25 @@ val bspec_chacha_quarter_round_post_tm =
  in
    bslSyntax.bandl [
     (snd o dest_eq o concl)
-     (EVAL ``bspec_var_equal_32_lowcast_64 "x20" ^a_exp``),
+     (EVAL ``bir_var_equal_32_lowcast_64 "x20" ^a_exp``),
     (snd o dest_eq o concl)
-     (EVAL ``bspec_var_equal_32_lowcast_64 "x21" ^b_exp``),
+     (EVAL ``bir_var_equal_32_lowcast_64 "x21" ^b_exp``),
     (snd o dest_eq o concl)
-     (EVAL ``bspec_var_equal_32_lowcast_64 "x8" ^c_exp``),
+     (EVAL ``bir_var_equal_32_lowcast_64 "x8" ^c_exp``),
     (snd o dest_eq o concl)
-     (EVAL ``bspec_var_equal_32_lowcast_64 "x22" ^d_exp``)
+     (EVAL ``bir_var_equal_32_lowcast_64 "x22" ^d_exp``)
    ]
  end;
 
-Definition bspec_chacha_quarter_round_post_def:
- bspec_chacha_quarter_round_post (pre_a:word32) (pre_b:word32)
+Definition bspec_chacha20_quarter_round_post_def:
+ bspec_chacha20_quarter_round_post (pre_a:word32) (pre_b:word32)
   (pre_c:word32) (pre_d:word32) : bir_exp_t =
-  ^bspec_chacha_quarter_round_post_tm
+  ^bspec_chacha20_quarter_round_post_tm
 End
 
 (* column round *)
 
-val bspec_chacha_column_round_pre_tm = bslSyntax.bandl [
+val bspec_chacha20_column_round_pre_tm = bslSyntax.bandl [
   ``BExp_BinPred
     BIExp_Equal
     (BExp_Cast BIExp_LowCast (BExp_Den (BVar "x10" (BType_Imm Bit64))) Bit32)
@@ -1134,20 +760,20 @@ val bspec_chacha_column_round_pre_tm = bslSyntax.bandl [
     (BExp_Const (Imm32 pre_arr_15))``
 ];
 
-Definition bspec_chacha_column_round_pre_def:
- bspec_chacha_column_round_pre 
+Definition bspec_chacha20_column_round_pre_def:
+ bspec_chacha20_column_round_pre 
   (pre_arr_0:word32) (pre_arr_1:word32) (pre_arr_2:word32) (pre_arr_3:word32)
   (pre_arr_4:word32) (pre_arr_5:word32) (pre_arr_6:word32) (pre_arr_7:word32) 
   (pre_arr_8:word32) (pre_arr_9:word32) (pre_arr_10:word32) (pre_arr_11:word32) 
   (pre_arr_12:word32) (pre_arr_13:word32) (pre_arr_14:word32) (pre_arr_15:word32) 
  : bir_exp_t =
-  ^bspec_chacha_column_round_pre_tm
+  ^bspec_chacha20_column_round_pre_tm
 End
 
-val bspec_chacha_column_round_post_tm =
+val bspec_chacha20_column_round_post_tm =
  let
    val bir_exprs = (snd o dest_eq o concl)
-    (EVAL ``bspec_chacha_column_round_bir_exprs 
+    (EVAL ``chacha_column_round_bir_exprs 
      (BExp_Const (Imm32 pre_arr_0))
      (BExp_Const (Imm32 pre_arr_1))
      (BExp_Const (Imm32 pre_arr_2))
@@ -1182,53 +808,53 @@ val bspec_chacha_column_round_post_tm =
  in
    bslSyntax.bandl [
     (snd o dest_eq o concl)
-     (EVAL ``bspec_var_equal_32_lowcast_64 "x20" ^arr_0_exp``),
+     (EVAL ``bir_var_equal_32_lowcast_64 "x20" ^arr_0_exp``),
     (snd o dest_eq o concl)
-     (EVAL ``bspec_var_equal_32_lowcast_64 "x19" ^arr_1_exp``),
+     (EVAL ``bir_var_equal_32_lowcast_64 "x19" ^arr_1_exp``),
     (snd o dest_eq o concl)
-     (EVAL ``bspec_var_equal_32_lowcast_64 "x18" ^arr_2_exp``),
+     (EVAL ``bir_var_equal_32_lowcast_64 "x18" ^arr_2_exp``),
     (snd o dest_eq o concl)
-     (EVAL ``bspec_var_equal_32_lowcast_64 "x9" ^arr_3_exp``),
+     (EVAL ``bir_var_equal_32_lowcast_64 "x9" ^arr_3_exp``),
     (snd o dest_eq o concl)
-     (EVAL ``bspec_var_equal_32_lowcast_64 "x21" ^arr_4_exp``),
+     (EVAL ``bir_var_equal_32_lowcast_64 "x21" ^arr_4_exp``),
     (snd o dest_eq o concl)
-     (EVAL ``bspec_var_equal_32_lowcast_64 "x10" ^arr_5_exp``),
+     (EVAL ``bir_var_equal_32_lowcast_64 "x10" ^arr_5_exp``),
     (snd o dest_eq o concl)
-     (EVAL ``bspec_var_equal_32_lowcast_64 "x13" ^arr_6_exp``),
+     (EVAL ``bir_var_equal_32_lowcast_64 "x13" ^arr_6_exp``),
     (snd o dest_eq o concl)
-     (EVAL ``bspec_var_equal_32_lowcast_64 "x14" ^arr_7_exp``),
+     (EVAL ``bir_var_equal_32_lowcast_64 "x14" ^arr_7_exp``),
     (snd o dest_eq o concl)
-     (EVAL ``bspec_var_equal_32_lowcast_64 "x8" ^arr_8_exp``),
+     (EVAL ``bir_var_equal_32_lowcast_64 "x8" ^arr_8_exp``),
     (snd o dest_eq o concl)
-     (EVAL ``bspec_var_equal_32_lowcast_64 "x7" ^arr_9_exp``),
+     (EVAL ``bir_var_equal_32_lowcast_64 "x7" ^arr_9_exp``),
     (snd o dest_eq o concl)
-     (EVAL ``bspec_var_equal_32_lowcast_64 "x5" ^arr_10_exp``),
+     (EVAL ``bir_var_equal_32_lowcast_64 "x5" ^arr_10_exp``),
     (snd o dest_eq o concl)
-     (EVAL ``bspec_var_equal_32_lowcast_64 "x15" ^arr_11_exp``),
+     (EVAL ``bir_var_equal_32_lowcast_64 "x15" ^arr_11_exp``),
     (snd o dest_eq o concl)
-     (EVAL ``bspec_var_equal_32_lowcast_64 "x22" ^arr_12_exp``),
+     (EVAL ``bir_var_equal_32_lowcast_64 "x22" ^arr_12_exp``),
     (snd o dest_eq o concl)
-     (EVAL ``bspec_var_equal_32_lowcast_64 "x28" ^arr_13_exp``),
+     (EVAL ``bir_var_equal_32_lowcast_64 "x28" ^arr_13_exp``),
     (snd o dest_eq o concl)
-     (EVAL ``bspec_var_equal_32_lowcast_64 "x29" ^arr_14_exp``),
+     (EVAL ``bir_var_equal_32_lowcast_64 "x29" ^arr_14_exp``),
     (snd o dest_eq o concl)
-     (EVAL ``bspec_var_equal_32_lowcast_64 "x16" ^arr_15_exp``)
+     (EVAL ``bir_var_equal_32_lowcast_64 "x16" ^arr_15_exp``)
    ]
  end;
 
-Definition bspec_chacha_column_round_post_def:
- bspec_chacha_column_round_post
+Definition bspec_chacha20_column_round_post_def:
+ bspec_chacha20_column_round_post
   (pre_arr_0:word32) (pre_arr_1:word32) (pre_arr_2:word32) (pre_arr_3:word32)
   (pre_arr_4:word32) (pre_arr_5:word32) (pre_arr_6:word32) (pre_arr_7:word32)
   (pre_arr_8:word32) (pre_arr_9:word32) (pre_arr_10:word32) (pre_arr_11:word32) 
   (pre_arr_12:word32) (pre_arr_13:word32) (pre_arr_14:word32) (pre_arr_15:word32)
  : bir_exp_t =
-  ^bspec_chacha_column_round_post_tm
+  ^bspec_chacha20_column_round_post_tm
 End
 
 (* diagonal round *)
 
-val bspec_chacha_diagonal_round_pre_tm = bslSyntax.bandl [
+val bspec_chacha20_diagonal_round_pre_tm = bslSyntax.bandl [
   ``BExp_BinPred
     BIExp_Equal
     (BExp_Cast BIExp_LowCast (BExp_Den (BVar "x20" (BType_Imm Bit64))) Bit32)
@@ -1295,20 +921,20 @@ val bspec_chacha_diagonal_round_pre_tm = bslSyntax.bandl [
     (BExp_Const (Imm32 pre_arr_15))``
 ];
 
-Definition bspec_chacha_diagonal_round_pre_def:
- bspec_chacha_diagonal_round_pre 
+Definition bspec_chacha20_diagonal_round_pre_def:
+ bspec_chacha20_diagonal_round_pre 
   (pre_arr_0:word32) (pre_arr_1:word32) (pre_arr_2:word32) (pre_arr_3:word32)
   (pre_arr_4:word32) (pre_arr_5:word32) (pre_arr_6:word32) (pre_arr_7:word32) 
   (pre_arr_8:word32) (pre_arr_9:word32) (pre_arr_10:word32) (pre_arr_11:word32) 
   (pre_arr_12:word32) (pre_arr_13:word32) (pre_arr_14:word32) (pre_arr_15:word32) 
  : bir_exp_t =
-  ^bspec_chacha_diagonal_round_pre_tm
+  ^bspec_chacha20_diagonal_round_pre_tm
 End
 
-val bspec_chacha_diagonal_round_post_tm =
+val bspec_chacha20_diagonal_round_post_tm =
  let
    val bir_exprs = (snd o dest_eq o concl)
-    (EVAL ``bspec_chacha_diagonal_round_bir_exprs 
+    (EVAL ``chacha_diagonal_round_bir_exprs 
      (BExp_Const (Imm32 pre_arr_0))
      (BExp_Const (Imm32 pre_arr_1))
      (BExp_Const (Imm32 pre_arr_2))
@@ -1343,53 +969,53 @@ val bspec_chacha_diagonal_round_post_tm =
  in
    bslSyntax.bandl [
     (snd o dest_eq o concl)
-     (EVAL ``bspec_var_equal_32_lowcast_64 "x10" ^arr_0_exp``),
+     (EVAL ``bir_var_equal_32_lowcast_64 "x10" ^arr_0_exp``),
     (snd o dest_eq o concl)
-     (EVAL ``bspec_var_equal_32_lowcast_64 "x16" ^arr_1_exp``),
+     (EVAL ``bir_var_equal_32_lowcast_64 "x16" ^arr_1_exp``),
     (snd o dest_eq o concl)
-     (EVAL ``bspec_var_equal_32_lowcast_64 "x17" ^arr_2_exp``),
+     (EVAL ``bir_var_equal_32_lowcast_64 "x17" ^arr_2_exp``),
     (snd o dest_eq o concl)
-     (EVAL ``bspec_var_equal_32_lowcast_64 "x6" ^arr_3_exp``),
+     (EVAL ``bir_var_equal_32_lowcast_64 "x6" ^arr_3_exp``),
     (snd o dest_eq o concl)
-     (EVAL ``bspec_var_equal_32_lowcast_64 "x22" ^arr_4_exp``),
+     (EVAL ``bir_var_equal_32_lowcast_64 "x22" ^arr_4_exp``),
     (snd o dest_eq o concl)
-     (EVAL ``bspec_var_equal_32_lowcast_64 "x11" ^arr_5_exp``),
+     (EVAL ``bir_var_equal_32_lowcast_64 "x11" ^arr_5_exp``),
     (snd o dest_eq o concl)
-     (EVAL ``bspec_var_equal_32_lowcast_64 "x13" ^arr_6_exp``),
+     (EVAL ``bir_var_equal_32_lowcast_64 "x13" ^arr_6_exp``),
     (snd o dest_eq o concl)
-     (EVAL ``bspec_var_equal_32_lowcast_64 "x14" ^arr_7_exp``),
+     (EVAL ``bir_var_equal_32_lowcast_64 "x14" ^arr_7_exp``),
     (snd o dest_eq o concl)
-     (EVAL ``bspec_var_equal_32_lowcast_64 "x28" ^arr_8_exp``),
+     (EVAL ``bir_var_equal_32_lowcast_64 "x28" ^arr_8_exp``),
     (snd o dest_eq o concl)
-     (EVAL ``bspec_var_equal_32_lowcast_64 "x29" ^arr_9_exp``),
+     (EVAL ``bir_var_equal_32_lowcast_64 "x29" ^arr_9_exp``),
     (snd o dest_eq o concl)
-     (EVAL ``bspec_var_equal_32_lowcast_64 "x30" ^arr_10_exp``),
+     (EVAL ``bir_var_equal_32_lowcast_64 "x30" ^arr_10_exp``),
     (snd o dest_eq o concl)
-     (EVAL ``bspec_var_equal_32_lowcast_64 "x31" ^arr_11_exp``),
+     (EVAL ``bir_var_equal_32_lowcast_64 "x31" ^arr_11_exp``),
     (snd o dest_eq o concl)
-     (EVAL ``bspec_var_equal_32_lowcast_64 "x26" ^arr_12_exp``),
+     (EVAL ``bir_var_equal_32_lowcast_64 "x26" ^arr_12_exp``),
     (snd o dest_eq o concl)
-     (EVAL ``bspec_var_equal_32_lowcast_64 "x25" ^arr_13_exp``),
+     (EVAL ``bir_var_equal_32_lowcast_64 "x25" ^arr_13_exp``),
     (snd o dest_eq o concl)
-     (EVAL ``bspec_var_equal_32_lowcast_64 "x24" ^arr_14_exp``),
+     (EVAL ``bir_var_equal_32_lowcast_64 "x24" ^arr_14_exp``),
     (snd o dest_eq o concl)
-     (EVAL ``bspec_var_equal_32_lowcast_64 "x23" ^arr_15_exp``)
+     (EVAL ``bir_var_equal_32_lowcast_64 "x23" ^arr_15_exp``)
    ]
  end;
 
-Definition bspec_chacha_diagonal_round_post_def:
- bspec_chacha_diagonal_round_post
+Definition bspec_chacha20_diagonal_round_post_def:
+ bspec_chacha20_diagonal_round_post
   (pre_arr_0:word32) (pre_arr_1:word32) (pre_arr_2:word32) (pre_arr_3:word32)
   (pre_arr_4:word32) (pre_arr_5:word32) (pre_arr_6:word32) (pre_arr_7:word32)
   (pre_arr_8:word32) (pre_arr_9:word32) (pre_arr_10:word32) (pre_arr_11:word32) 
   (pre_arr_12:word32) (pre_arr_13:word32) (pre_arr_14:word32) (pre_arr_15:word32)
  : bir_exp_t =
-  ^bspec_chacha_diagonal_round_post_tm
+  ^bspec_chacha20_diagonal_round_post_tm
 End
 
 (* double round *)
 
-val bspec_chacha_double_round_pre_tm = bslSyntax.bandl [
+val bspec_chacha20_double_round_pre_tm = bslSyntax.bandl [
   ``BExp_BinPred
     BIExp_Equal
     (BExp_Cast BIExp_LowCast (BExp_Den (BVar "x10" (BType_Imm Bit64))) Bit32)
@@ -1456,20 +1082,20 @@ val bspec_chacha_double_round_pre_tm = bslSyntax.bandl [
     (BExp_Const (Imm32 pre_arr_15))``
 ];
 
-Definition bspec_chacha_double_round_pre_def:
- bspec_chacha_double_round_pre 
+Definition bspec_chacha20_double_round_pre_def:
+ bspec_chacha20_double_round_pre 
   (pre_arr_0:word32) (pre_arr_1:word32) (pre_arr_2:word32) (pre_arr_3:word32)
   (pre_arr_4:word32) (pre_arr_5:word32) (pre_arr_6:word32) (pre_arr_7:word32) 
   (pre_arr_8:word32) (pre_arr_9:word32) (pre_arr_10:word32) (pre_arr_11:word32) 
   (pre_arr_12:word32) (pre_arr_13:word32) (pre_arr_14:word32) (pre_arr_15:word32) 
  : bir_exp_t =
-  ^bspec_chacha_double_round_pre_tm
+  ^bspec_chacha20_double_round_pre_tm
 End
 
-val bspec_chacha_double_round_post_tm =
+val bspec_chacha20_double_round_post_tm =
  let
    val bir_exprs = (snd o dest_eq o concl)
-    (EVAL ``bspec_chacha_round_bir_exprs 
+    (EVAL ``chacha_double_round_bir_exprs 
      (BExp_Const (Imm32 pre_arr_0))
      (BExp_Const (Imm32 pre_arr_1))
      (BExp_Const (Imm32 pre_arr_2))
@@ -1504,18 +1130,48 @@ val bspec_chacha_double_round_post_tm =
  in
    bslSyntax.bandl [
     (snd o dest_eq o concl)
-     (EVAL ``bspec_var_equal_32_lowcast_64 "x10" ^arr_0_exp``)
+     (EVAL ``bir_var_equal_32_lowcast_64 "x10" ^arr_0_exp``),
+    (snd o dest_eq o concl)
+     (EVAL ``bir_var_equal_32_lowcast_64 "x16" ^arr_1_exp``),
+    (snd o dest_eq o concl)
+     (EVAL ``bir_var_equal_32_lowcast_64 "x17" ^arr_2_exp``),
+    (snd o dest_eq o concl)
+     (EVAL ``bir_var_equal_32_lowcast_64 "x6" ^arr_3_exp``),
+    (snd o dest_eq o concl)
+     (EVAL ``bir_var_equal_32_lowcast_64 "x22" ^arr_4_exp``),
+    (snd o dest_eq o concl)
+     (EVAL ``bir_var_equal_32_lowcast_64 "x11" ^arr_5_exp``),
+    (snd o dest_eq o concl)
+     (EVAL ``bir_var_equal_32_lowcast_64 "x13" ^arr_6_exp``),
+    (snd o dest_eq o concl)
+     (EVAL ``bir_var_equal_32_lowcast_64 "x14" ^arr_7_exp``),
+    (snd o dest_eq o concl)
+     (EVAL ``bir_var_equal_32_lowcast_64 "x28" ^arr_8_exp``),
+    (snd o dest_eq o concl)
+     (EVAL ``bir_var_equal_32_lowcast_64 "x29" ^arr_9_exp``),
+    (snd o dest_eq o concl)
+     (EVAL ``bir_var_equal_32_lowcast_64 "x30" ^arr_10_exp``),
+    (snd o dest_eq o concl)
+     (EVAL ``bir_var_equal_32_lowcast_64 "x31" ^arr_11_exp``),
+    (snd o dest_eq o concl)
+     (EVAL ``bir_var_equal_32_lowcast_64 "x26" ^arr_12_exp``),
+    (snd o dest_eq o concl)
+     (EVAL ``bir_var_equal_32_lowcast_64 "x25" ^arr_13_exp``),
+    (snd o dest_eq o concl)
+     (EVAL ``bir_var_equal_32_lowcast_64 "x24" ^arr_14_exp``),
+    (snd o dest_eq o concl)
+     (EVAL ``bir_var_equal_32_lowcast_64 "x23" ^arr_15_exp``)
    ]
  end;
 
-Definition bspec_chacha_double_round_post_def:
- bspec_chacha_double_round_post
+Definition bspec_chacha20_double_round_post_def:
+ bspec_chacha20_double_round_post
   (pre_arr_0:word32) (pre_arr_1:word32) (pre_arr_2:word32) (pre_arr_3:word32)
   (pre_arr_4:word32) (pre_arr_5:word32) (pre_arr_6:word32) (pre_arr_7:word32)
   (pre_arr_8:word32) (pre_arr_9:word32) (pre_arr_10:word32) (pre_arr_11:word32) 
   (pre_arr_12:word32) (pre_arr_13:word32) (pre_arr_14:word32) (pre_arr_15:word32)
  : bir_exp_t =
-  ^bspec_chacha_double_round_post_tm
+  ^bspec_chacha20_double_round_post_tm
 End
 
 val _ = export_theory ();
