examples/riscv/chacha20/chacha20_column_round_symb_execScript.sml
@@ -4,15 +4,15 @@ open wordsTheory;
 
 open bir_symbLib;
 
-open chachaTheory chacha_specTheory;
+open chacha20Theory chacha20_specTheory;
 
-val _ = new_theory "chacha_symb_exec_column_round";
+val _ = new_theory "chacha20_column_round_symb_exec";
 
 (* --------------------------- *)
 (* prepare program lookups     *)
 (* --------------------------- *)
 
-val bir_lift_thm = bir_chacha_riscv_lift_THM;
+val bir_lift_thm = bir_chacha20_riscv_lift_THM;
 val _ = birs_auxLib.prepare_program_lookups bir_lift_thm;
 
 (* --------------------------- *)
@@ -27,12 +27,12 @@ val _ = show_tags := true;
 
 val symb_analysis_thm =
  bir_symb_analysis_thm
-  bir_chacha_prog_def
-  chacha_column_round_init_addr_def [chacha_column_round_end_addr_def]
-  bspec_chacha_column_round_pre_def chacha_birenvtyl_def;
+  bir_chacha20_prog_def
+  chacha20_column_round_init_addr_def [chacha20_column_round_end_addr_def]
+  bspec_chacha20_column_round_pre_def chacha20_birenvtyl_def;
 
 val _ = Portable.pprint Tag.pp_tag (tag symb_analysis_thm);
 
-Theorem chacha_column_round_symb_analysis_thm = symb_analysis_thm
+Theorem chacha20_column_round_symb_analysis_thm = symb_analysis_thm
 
 val _ = export_theory ();
