examples/riscv/chacha20/chacha20_quarter_round_symb_execScript.sml
@@ -4,15 +4,15 @@ open wordsTheory;
 
 open bir_symbLib;
 
-open chachaTheory chacha_specTheory;
+open chacha20Theory chacha20_specTheory;
 
-val _ = new_theory "chacha_symb_exec_quarter_round";
+val _ = new_theory "chacha20_quarter_round_symb_exec";
 
 (* --------------------------- *)
 (* prepare program lookups     *)
 (* --------------------------- *)
 
-val bir_lift_thm = bir_chacha_riscv_lift_THM;
+val bir_lift_thm = bir_chacha20_riscv_lift_THM;
 val _ = birs_auxLib.prepare_program_lookups bir_lift_thm;
 
 (* --------------------------- *)
@@ -27,13 +27,13 @@ val _ = show_tags := true;
 
 val symb_analysis_thm =
  bir_symb_analysis_thm
-  bir_chacha_prog_def
-  chacha_line_init_addr_def [chacha_line_end_addr_def]
-  bspec_chacha_line_pre_def chacha_birenvtyl_def;
+  bir_chacha20_prog_def
+  chacha20_line_init_addr_def [chacha20_line_end_addr_def]
+  bspec_chacha20_line_pre_def chacha20_birenvtyl_def;
 
 val _ = Portable.pprint Tag.pp_tag (tag symb_analysis_thm);
 
-Theorem chacha_line_symb_analysis_thm = symb_analysis_thm
+Theorem chacha20_line_symb_analysis_thm = symb_analysis_thm
 
 (* ----------- *)
 (* second line *)
@@ -41,13 +41,13 @@ Theorem chacha_line_symb_analysis_thm = symb_analysis_thm
 
 val symb_analysis_thm =
  bir_symb_analysis_thm
-  bir_chacha_prog_def
-  chacha_other_line_init_addr_def [chacha_other_line_end_addr_def]
-  bspec_chacha_line_pre_other_def chacha_birenvtyl_def;
+  bir_chacha20_prog_def
+  chacha20_other_line_init_addr_def [chacha20_other_line_end_addr_def]
+  bspec_chacha20_line_pre_other_def chacha20_birenvtyl_def;
 
 val _ = Portable.pprint Tag.pp_tag (tag symb_analysis_thm);
 
-Theorem chacha_other_line_symb_analysis_thm = symb_analysis_thm
+Theorem chacha20_other_line_symb_analysis_thm = symb_analysis_thm
 
 (* ------------------- *)
 (* first quarter round *)
@@ -55,12 +55,12 @@ Theorem chacha_other_line_symb_analysis_thm = symb_analysis_thm
 
 val symb_analysis_thm =
  bir_symb_analysis_thm
-  bir_chacha_prog_def
-  chacha_quarter_round_init_addr_def [chacha_quarter_round_end_addr_def]
-  bspec_chacha_quarter_round_pre_def chacha_birenvtyl_def;
+  bir_chacha20_prog_def
+  chacha20_quarter_round_init_addr_def [chacha20_quarter_round_end_addr_def]
+  bspec_chacha20_quarter_round_pre_def chacha20_birenvtyl_def;
 
 val _ = Portable.pprint Tag.pp_tag (tag symb_analysis_thm);
 
-Theorem chacha_quarter_round_symb_analysis_thm = symb_analysis_thm
+Theorem chacha20_quarter_round_symb_analysis_thm = symb_analysis_thm
 
 val _ = export_theory ();
